session.v
@@ -376,8 +376,14 @@ Qed.
 
 End Session.
 
+Definition sessionΣ : gFunctor :=
+  GFunctor sessionR.
+
 Arguments sessionG Σ : clear implicits.
 Arguments session_alloc {Σ _} term_meta {X _ _ _} N P.
 Arguments session_begin {Σ _ _ _ _ _ _ _ _}  {N P} E γ rl tI tR.
 Arguments session_ctx {Σ _} term_meta {_ _ _ _} N P γ.
 Arguments session {Σ} term_meta {_ _ _ _} N γ _ _ _.
+
+Instance subG_sessionΣ {Σ} : subG sessionΣ Σ → sessionG Σ.
+Proof. solve_inG. Qed.
